projects/lib/gmp_goal.v
@@ -1787,6 +1787,8 @@ forall (b_pre: Z) (n_pre: Z) (ap_pre: Z) (rp_pre: Z) (cap2: Z) (cap1: Z) (l2: (@
   &&  [| (i < n_pre) |] 
   &&  [| (n_pre <= cap2) |] 
   &&  [| ((unsigned_last_nbits (((Znth i l_2 0) + b )) (32)) >= b) |] 
+  &&  [| (0 <= b) |] 
+  &&  [| (b <= UINT_MAX) |] 
   &&  [| (i < n_pre) |] 
   &&  [| (0 <= i) |] 
   &&  [| (i <= n_pre) |] 
@@ -1810,10 +1812,10 @@ forall (b_pre: Z) (n_pre: Z) (ap_pre: Z) (rp_pre: Z) (cap2: Z) (cap1: Z) (l2: (@
   &&  (store_uint_array rp_pre (i + 1 ) (replace_Znth (i) ((unsigned_last_nbits (((Znth i l_2 0) + b )) (32))) ((app (l') ((cons (a) (nil)))))) )
   **  ((( &( "i" ) )) # Int  |-> i)
   **  (store_uint_array_rec rp_pre (i + 1 ) cap2 l''' )
+  **  ((( &( "b" ) )) # UInt  |-> 0)
   **  (store_uint_array ap_pre n_pre l_2 )
   **  ((( &( "r" ) )) # UInt  |-> (unsigned_last_nbits (((Znth i l_2 0) + b )) (32)))
   **  (store_undef_uint_array_rec ap_pre n_pre cap1 )
-  **  ((( &( "b" ) )) # UInt  |-> 0)
   **  ((( &( "n" ) )) # Int  |-> n_pre)
   **  ((( &( "ap" ) )) # Ptr  |-> ap_pre)
   **  ((( &( "rp" ) )) # Ptr  |-> rp_pre)
@@ -1829,6 +1831,8 @@ forall (b_pre: Z) (n_pre: Z) (ap_pre: Z) (rp_pre: Z) (cap2: Z) (cap1: Z) (l2: (@
   &&  [| (i < n_pre) |] 
   &&  [| (n_pre <= cap2) |] 
   &&  [| ((unsigned_last_nbits (((Znth i l_2 0) + b )) (32)) < b) |] 
+  &&  [| (0 <= b) |] 
+  &&  [| (b <= UINT_MAX) |] 
   &&  [| (i < n_pre) |] 
   &&  [| (0 <= i) |] 
   &&  [| (i <= n_pre) |] 
@@ -1852,10 +1856,10 @@ forall (b_pre: Z) (n_pre: Z) (ap_pre: Z) (rp_pre: Z) (cap2: Z) (cap1: Z) (l2: (@
   &&  (store_uint_array rp_pre (i + 1 ) (replace_Znth (i) ((unsigned_last_nbits (((Znth i l_2 0) + b )) (32))) ((app (l') ((cons (a) (nil)))))) )
   **  ((( &( "i" ) )) # Int  |-> i)
   **  (store_uint_array_rec rp_pre (i + 1 ) cap2 l''' )
+  **  ((( &( "b" ) )) # UInt  |-> 1)
   **  (store_uint_array ap_pre n_pre l_2 )
   **  ((( &( "r" ) )) # UInt  |-> (unsigned_last_nbits (((Znth i l_2 0) + b )) (32)))
   **  (store_undef_uint_array_rec ap_pre n_pre cap1 )
-  **  ((( &( "b" ) )) # UInt  |-> 1)
   **  ((( &( "n" ) )) # Int  |-> n_pre)
   **  ((( &( "ap" ) )) # Ptr  |-> ap_pre)
   **  ((( &( "rp" ) )) # Ptr  |-> rp_pre)
@@ -1908,13 +1912,82 @@ forall (b_pre: Z) (n_pre: Z) (ap_pre: Z) (rp_pre: Z) (cap2: Z) (cap1: Z) (l2: (@
   **  (store_uint_array_rec rp_pre 0 cap2 l'' )
 .
 
-Definition mpn_add_1_entail_wit_2_1 := 
+Definition mpn_add_1_entail_wit_2 := 
+forall (b_pre: Z) (n_pre: Z) (ap_pre: Z) (rp_pre: Z) (cap2: Z) (cap1: Z) (l2: (@list Z)) (val: Z) (l: (@list Z)) (b: Z) (l'': (@list Z)) (l': (@list Z)) (val2: Z) (val1: Z) (l_2: (@list Z)) (i: Z) ,
+  [| (i < n_pre) |] 
+  &&  [| (0 <= i) |] 
+  &&  [| (i <= n_pre) |] 
+  &&  [| (list_store_Z_compact l_2 val ) |] 
+  &&  [| (n_pre <= cap1) |] 
+  &&  [| (list_store_Z (sublist (0) (i) (l_2)) val1 ) |] 
+  &&  [| (list_store_Z l' val2 ) |] 
+  &&  [| ((val2 + (b * (Z.pow (UINT_MOD) (i)) ) ) = (val1 + b_pre )) |] 
+  &&  [| ((Zlength (l')) = i) |] 
+  &&  [| ((Zlength (l2)) = cap2) |] 
+  &&  [| (n_pre <= cap1) |] 
+  &&  [| ((Zlength (l)) = n_pre) |] 
+  &&  [| (cap1 <= 100000000) |] 
+  &&  [| (list_store_Z_compact l val ) |] 
+  &&  [| ((Zlength (l2)) = cap2) |] 
+  &&  [| (cap2 >= n_pre) |] 
+  &&  [| (cap1 <= 100000000) |] 
+  &&  [| (cap2 <= 100000000) |] 
+  &&  [| (n_pre > 0) |] 
+  &&  [| (n_pre <= cap1) |]
+  &&  (store_uint_array ap_pre n_pre l_2 )
+  **  ((( &( "r" ) )) # UInt  |-> (unsigned_last_nbits (((Znth i l_2 0) + b )) (32)))
+  **  ((( &( "i" ) )) # Int  |-> i)
+  **  (store_undef_uint_array_rec ap_pre n_pre cap1 )
+  **  (store_uint_array rp_pre i l' )
+  **  (store_uint_array_rec rp_pre i cap2 l'' )
+  **  ((( &( "b" ) )) # UInt  |-> b)
+  **  ((( &( "n" ) )) # Int  |-> n_pre)
+  **  ((( &( "ap" ) )) # Ptr  |-> ap_pre)
+  **  ((( &( "rp" ) )) # Ptr  |-> rp_pre)
+|--
+  [| (0 <= b) |] 
+  &&  [| (b <= UINT_MAX) |] 
+  &&  [| (i < n_pre) |] 
+  &&  [| (0 <= i) |] 
+  &&  [| (i <= n_pre) |] 
+  &&  [| (list_store_Z_compact l_2 val ) |] 
+  &&  [| (n_pre <= cap1) |] 
+  &&  [| (list_store_Z (sublist (0) (i) (l_2)) val1 ) |] 
+  &&  [| (list_store_Z l' val2 ) |] 
+  &&  [| ((val2 + (b * (Z.pow (UINT_MOD) (i)) ) ) = (val1 + b_pre )) |] 
+  &&  [| ((Zlength (l')) = i) |] 
+  &&  [| ((Zlength (l2)) = cap2) |] 
+  &&  [| (n_pre <= cap1) |] 
+  &&  [| ((Zlength (l)) = n_pre) |] 
+  &&  [| (cap1 <= 100000000) |] 
+  &&  [| (list_store_Z_compact l val ) |] 
+  &&  [| ((Zlength (l2)) = cap2) |] 
+  &&  [| (cap2 >= n_pre) |] 
+  &&  [| (cap1 <= 100000000) |] 
+  &&  [| (cap2 <= 100000000) |] 
+  &&  [| (n_pre > 0) |] 
+  &&  [| (n_pre <= cap1) |]
+  &&  ((( &( "b" ) )) # UInt  |-> b)
+  **  (store_uint_array ap_pre n_pre l_2 )
+  **  ((( &( "r" ) )) # UInt  |-> (unsigned_last_nbits (((Znth i l_2 0) + b )) (32)))
+  **  ((( &( "i" ) )) # Int  |-> i)
+  **  (store_undef_uint_array_rec ap_pre n_pre cap1 )
+  **  (store_uint_array rp_pre i l' )
+  **  (store_uint_array_rec rp_pre i cap2 l'' )
+  **  ((( &( "n" ) )) # Int  |-> n_pre)
+  **  ((( &( "ap" ) )) # Ptr  |-> ap_pre)
+  **  ((( &( "rp" ) )) # Ptr  |-> rp_pre)
+.
+
+Definition mpn_add_1_entail_wit_3_1 := 
 forall (b_pre: Z) (n_pre: Z) (ap_pre: Z) (rp_pre: Z) (cap2: Z) (cap1: Z) (l2: (@list Z)) (val: Z) (l_2: (@list Z)) (b: Z) (l''_2: (@list Z)) (l'_2: (@list Z)) (val2_2: Z) (val1_2: Z) (l_3: (@list Z)) (i: Z) (a: Z) (l''': (@list Z)) ,
   [| (l''_2 = (cons (a) (l'''))) |] 
   &&  [| (0 <= i) |] 
   &&  [| (i < n_pre) |] 
   &&  [| (n_pre <= cap2) |] 
   &&  [| ((unsigned_last_nbits (((Znth i l_3 0) + b )) (32)) < b) |] 
+  &&  [| (0 <= b) |] 
+  &&  [| (b <= UINT_MAX) |] 
   &&  [| (i < n_pre) |] 
   &&  [| (0 <= i) |] 
   &&  [| (i <= n_pre) |] 
@@ -1966,13 +2039,15 @@ forall (b_pre: Z) (n_pre: Z) (ap_pre: Z) (rp_pre: Z) (cap2: Z) (cap1: Z) (l2: (@
   **  (store_uint_array_rec rp_pre (i + 1 ) cap2 l'' )
 .
 
-Definition mpn_add_1_entail_wit_2_2 := 
+Definition mpn_add_1_entail_wit_3_2 := 
 forall (b_pre: Z) (n_pre: Z) (ap_pre: Z) (rp_pre: Z) (cap2: Z) (cap1: Z) (l2: (@list Z)) (val: Z) (l_2: (@list Z)) (b: Z) (l''_2: (@list Z)) (l'_2: (@list Z)) (val2_2: Z) (val1_2: Z) (l_3: (@list Z)) (i: Z) (a: Z) (l''': (@list Z)) ,
   [| (l''_2 = (cons (a) (l'''))) |] 
   &&  [| (0 <= i) |] 
   &&  [| (i < n_pre) |] 
   &&  [| (n_pre <= cap2) |] 
   &&  [| ((unsigned_last_nbits (((Znth i l_3 0) + b )) (32)) >= b) |] 
+  &&  [| (0 <= b) |] 
+  &&  [| (b <= UINT_MAX) |] 
   &&  [| (i < n_pre) |] 
   &&  [| (0 <= i) |] 
   &&  [| (i <= n_pre) |] 
@@ -2193,6 +2268,8 @@ forall (b_pre: Z) (n_pre: Z) (ap_pre: Z) (rp_pre: Z) (cap2: Z) (cap1: Z) (l2: (@
 Definition mpn_add_1_partial_solve_wit_4_pure := 
 forall (b_pre: Z) (n_pre: Z) (ap_pre: Z) (rp_pre: Z) (cap2: Z) (cap1: Z) (l2: (@list Z)) (val: Z) (l: (@list Z)) (b: Z) (l'': (@list Z)) (l': (@list Z)) (val2: Z) (val1: Z) (l_2: (@list Z)) (i: Z) ,
   [| ((unsigned_last_nbits (((Znth i l_2 0) + b )) (32)) >= b) |] 
+  &&  [| (0 <= b) |] 
+  &&  [| (b <= UINT_MAX) |] 
   &&  [| (i < n_pre) |] 
   &&  [| (0 <= i) |] 
   &&  [| (i <= n_pre) |] 
@@ -2213,13 +2290,13 @@ forall (b_pre: Z) (n_pre: Z) (ap_pre: Z) (rp_pre: Z) (cap2: Z) (cap1: Z) (l2: (@
   &&  [| (cap2 <= 100000000) |] 
   &&  [| (n_pre > 0) |] 
   &&  [| (n_pre <= cap1) |]
-  &&  (store_uint_array ap_pre n_pre l_2 )
+  &&  ((( &( "b" ) )) # UInt  |-> 0)
+  **  (store_uint_array ap_pre n_pre l_2 )
   **  ((( &( "r" ) )) # UInt  |-> (unsigned_last_nbits (((Znth i l_2 0) + b )) (32)))
   **  ((( &( "i" ) )) # Int  |-> i)
   **  (store_undef_uint_array_rec ap_pre n_pre cap1 )
   **  (store_uint_array rp_pre i l' )
   **  (store_uint_array_rec rp_pre i cap2 l'' )
-  **  ((( &( "b" ) )) # UInt  |-> 0)
   **  ((( &( "n" ) )) # Int  |-> n_pre)
   **  ((( &( "ap" ) )) # Ptr  |-> ap_pre)
   **  ((( &( "rp" ) )) # Ptr  |-> rp_pre)
@@ -2232,6 +2309,8 @@ forall (b_pre: Z) (n_pre: Z) (ap_pre: Z) (rp_pre: Z) (cap2: Z) (cap1: Z) (l2: (@
 Definition mpn_add_1_partial_solve_wit_4_aux := 
 forall (b_pre: Z) (n_pre: Z) (ap_pre: Z) (rp_pre: Z) (cap2: Z) (cap1: Z) (l2: (@list Z)) (val: Z) (l: (@list Z)) (b: Z) (l'': (@list Z)) (l': (@list Z)) (val2: Z) (val1: Z) (l_2: (@list Z)) (i: Z) ,
   [| ((unsigned_last_nbits (((Znth i l_2 0) + b )) (32)) >= b) |] 
+  &&  [| (0 <= b) |] 
+  &&  [| (b <= UINT_MAX) |] 
   &&  [| (i < n_pre) |] 
   &&  [| (0 <= i) |] 
   &&  [| (i <= n_pre) |] 
@@ -2261,6 +2340,8 @@ forall (b_pre: Z) (n_pre: Z) (ap_pre: Z) (rp_pre: Z) (cap2: Z) (cap1: Z) (l2: (@
   &&  [| (i < n_pre) |] 
   &&  [| (n_pre <= cap2) |] 
   &&  [| ((unsigned_last_nbits (((Znth i l_2 0) + b )) (32)) >= b) |] 
+  &&  [| (0 <= b) |] 
+  &&  [| (b <= UINT_MAX) |] 
   &&  [| (i < n_pre) |] 
   &&  [| (0 <= i) |] 
   &&  [| (i <= n_pre) |] 
@@ -2292,6 +2373,8 @@ Definition mpn_add_1_partial_solve_wit_4 := mpn_add_1_partial_solve_wit_4_pure -
 Definition mpn_add_1_partial_solve_wit_5_pure := 
 forall (b_pre: Z) (n_pre: Z) (ap_pre: Z) (rp_pre: Z) (cap2: Z) (cap1: Z) (l2: (@list Z)) (val: Z) (l: (@list Z)) (b: Z) (l'': (@list Z)) (l': (@list Z)) (val2: Z) (val1: Z) (l_2: (@list Z)) (i: Z) ,
   [| ((unsigned_last_nbits (((Znth i l_2 0) + b )) (32)) < b) |] 
+  &&  [| (0 <= b) |] 
+  &&  [| (b <= UINT_MAX) |] 
   &&  [| (i < n_pre) |] 
   &&  [| (0 <= i) |] 
   &&  [| (i <= n_pre) |] 
@@ -2312,13 +2395,13 @@ forall (b_pre: Z) (n_pre: Z) (ap_pre: Z) (rp_pre: Z) (cap2: Z) (cap1: Z) (l2: (@
   &&  [| (cap2 <= 100000000) |] 
   &&  [| (n_pre > 0) |] 
   &&  [| (n_pre <= cap1) |]
-  &&  (store_uint_array ap_pre n_pre l_2 )
+  &&  ((( &( "b" ) )) # UInt  |-> 1)
+  **  (store_uint_array ap_pre n_pre l_2 )
   **  ((( &( "r" ) )) # UInt  |-> (unsigned_last_nbits (((Znth i l_2 0) + b )) (32)))
   **  ((( &( "i" ) )) # Int  |-> i)
   **  (store_undef_uint_array_rec ap_pre n_pre cap1 )
   **  (store_uint_array rp_pre i l' )
   **  (store_uint_array_rec rp_pre i cap2 l'' )
-  **  ((( &( "b" ) )) # UInt  |-> 1)
   **  ((( &( "n" ) )) # Int  |-> n_pre)
   **  ((( &( "ap" ) )) # Ptr  |-> ap_pre)
   **  ((( &( "rp" ) )) # Ptr  |-> rp_pre)
@@ -2331,6 +2414,8 @@ forall (b_pre: Z) (n_pre: Z) (ap_pre: Z) (rp_pre: Z) (cap2: Z) (cap1: Z) (l2: (@
 Definition mpn_add_1_partial_solve_wit_5_aux := 
 forall (b_pre: Z) (n_pre: Z) (ap_pre: Z) (rp_pre: Z) (cap2: Z) (cap1: Z) (l2: (@list Z)) (val: Z) (l: (@list Z)) (b: Z) (l'': (@list Z)) (l': (@list Z)) (val2: Z) (val1: Z) (l_2: (@list Z)) (i: Z) ,
   [| ((unsigned_last_nbits (((Znth i l_2 0) + b )) (32)) < b) |] 
+  &&  [| (0 <= b) |] 
+  &&  [| (b <= UINT_MAX) |] 
   &&  [| (i < n_pre) |] 
   &&  [| (0 <= i) |] 
   &&  [| (i <= n_pre) |] 
@@ -2360,6 +2445,8 @@ forall (b_pre: Z) (n_pre: Z) (ap_pre: Z) (rp_pre: Z) (cap2: Z) (cap1: Z) (l2: (@
   &&  [| (i < n_pre) |] 
   &&  [| (n_pre <= cap2) |] 
   &&  [| ((unsigned_last_nbits (((Znth i l_2 0) + b )) (32)) < b) |] 
+  &&  [| (0 <= b) |] 
+  &&  [| (b <= UINT_MAX) |] 
   &&  [| (i < n_pre) |] 
   &&  [| (0 <= i) |] 
   &&  [| (i <= n_pre) |] 
@@ -2395,6 +2482,8 @@ forall (b_pre: Z) (n_pre: Z) (ap_pre: Z) (rp_pre: Z) (cap2: Z) (cap1: Z) (l2: (@
   &&  [| (i < n_pre) |] 
   &&  [| (n_pre <= cap2) |] 
   &&  [| ((unsigned_last_nbits (((Znth i l_2 0) + b )) (32)) < b) |] 
+  &&  [| (0 <= b) |] 
+  &&  [| (b <= UINT_MAX) |] 
   &&  [| (i < n_pre) |] 
   &&  [| (0 <= i) |] 
   &&  [| (i <= n_pre) |] 
@@ -2425,6 +2514,8 @@ forall (b_pre: Z) (n_pre: Z) (ap_pre: Z) (rp_pre: Z) (cap2: Z) (cap1: Z) (l2: (@
   &&  [| (i < n_pre) |] 
   &&  [| (n_pre <= cap2) |] 
   &&  [| ((unsigned_last_nbits (((Znth i l_2 0) + b )) (32)) < b) |] 
+  &&  [| (0 <= b) |] 
+  &&  [| (b <= UINT_MAX) |] 
   &&  [| (i < n_pre) |] 
   &&  [| (0 <= i) |] 
   &&  [| (i <= n_pre) |] 
@@ -2459,6 +2550,8 @@ forall (b_pre: Z) (n_pre: Z) (ap_pre: Z) (rp_pre: Z) (cap2: Z) (cap1: Z) (l2: (@
   &&  [| (i < n_pre) |] 
   &&  [| (n_pre <= cap2) |] 
   &&  [| ((unsigned_last_nbits (((Znth i l_2 0) + b )) (32)) >= b) |] 
+  &&  [| (0 <= b) |] 
+  &&  [| (b <= UINT_MAX) |] 
   &&  [| (i < n_pre) |] 
   &&  [| (0 <= i) |] 
   &&  [| (i <= n_pre) |] 
@@ -2489,6 +2582,8 @@ forall (b_pre: Z) (n_pre: Z) (ap_pre: Z) (rp_pre: Z) (cap2: Z) (cap1: Z) (l2: (@
   &&  [| (i < n_pre) |] 
   &&  [| (n_pre <= cap2) |] 
   &&  [| ((unsigned_last_nbits (((Znth i l_2 0) + b )) (32)) >= b) |] 
+  &&  [| (0 <= b) |] 
+  &&  [| (b <= UINT_MAX) |] 
   &&  [| (i < n_pre) |] 
   &&  [| (0 <= i) |] 
   &&  [| (i <= n_pre) |] 
@@ -2630,8 +2725,9 @@ Axiom proof_of_mpn_add_1_safety_wit_1 : mpn_add_1_safety_wit_1.
 Axiom proof_of_mpn_add_1_safety_wit_2 : mpn_add_1_safety_wit_2.
 Axiom proof_of_mpn_add_1_safety_wit_3 : mpn_add_1_safety_wit_3.
 Axiom proof_of_mpn_add_1_entail_wit_1 : mpn_add_1_entail_wit_1.
-Axiom proof_of_mpn_add_1_entail_wit_2_1 : mpn_add_1_entail_wit_2_1.
-Axiom proof_of_mpn_add_1_entail_wit_2_2 : mpn_add_1_entail_wit_2_2.
+Axiom proof_of_mpn_add_1_entail_wit_2 : mpn_add_1_entail_wit_2.
+Axiom proof_of_mpn_add_1_entail_wit_3_1 : mpn_add_1_entail_wit_3_1.
+Axiom proof_of_mpn_add_1_entail_wit_3_2 : mpn_add_1_entail_wit_3_2.
 Axiom proof_of_mpn_add_1_return_wit_1 : mpn_add_1_return_wit_1.
 Axiom proof_of_mpn_add_1_partial_solve_wit_1 : mpn_add_1_partial_solve_wit_1.
 Axiom proof_of_mpn_add_1_partial_solve_wit_2_pure : mpn_add_1_partial_solve_wit_2_pure.
